Added bank code and basic definitions for bank proof

src/program_proof/lockservice/kv_proof.v
@@ -13,47 +13,52 @@ From Perennial.Helpers Require Import NamedProps.
 From Perennial.Helpers Require Import ModArith.
 From Perennial.program_proof.lockservice Require Import lockservice fmcounter_map rpc common_proof nondet rpc.
 
+Record kvservice_names := KVserviceGN {
+  ks_rpcGN : rpc_names;
+  ks_kvMapGN : gname;
+}.
+
+Class kvserviceG Σ := KVserviceG {
+  ls_rpcG :> rpcG Σ u64; (* RPC layer ghost state *)
+  ls_kvMapG :> mapG Σ u64 u64; (* [γkv]: tracks the state of the KV server *logically* *)
+}.
+
 Section kv_proof.
-Context `{!heapG Σ}.
+Context `{!heapG Σ, !kvserviceG Σ}.
 
-Implicit Types s : Slice.t.
-Implicit Types (stk:stuckness) (E: coPset).
-
-  Context `{!rpcG Σ u64}.
-  Context `{!mapG Σ (u64*u64) unit}.
-  Context `{!mapG Σ u64 u64}.
-
-  Context `{γkv:gname}.
+Implicit Types (γ : kvservice_names).
 
 Local Notation "k [[ γ ]]↦ '_'" := (∃ v, k [[γ]]↦ v)%I
 (at level 20, format "k  [[ γ ]]↦ '_'") : bi_scope.
 
+(*
 Definition Get_Pre : u64 -> iProp Σ := (λ k, k [[γkv]]↦ _)%I.
 Definition Get_Post : u64 -> u64 -> iProp Σ := λ k v, (k [[γkv]]↦ v)%I.
 
 Definition Put_Pre : u64 -> u64 -> iProp Σ := (λ k _, k [[γkv]]↦ _)%I.
 Definition Put_Post : u64 -> u64 -> iProp Σ := (λ k v, k [[γkv]]↦ v)%I.
+*)
 
-Definition KVServer_own_core (srv:loc) : iProp Σ :=
+Definition KVServer_own_core γ (srv:loc) : iProp Σ :=
   ∃ (kvs_ptr:loc) (kvsM:gmap u64 u64),
   "HlocksOwn" ∷ srv ↦[KVServer.S :: "kvs"] #kvs_ptr
 ∗ "HkvsMap" ∷ is_map (kvs_ptr) kvsM
-∗ "Hkvctx" ∷ map_ctx γkv 1 kvsM
+∗ "Hkvctx" ∷ map_ctx γ.(ks_kvMapGN) 1 kvsM
 .
 
 (* FIXME: this is currently just a placeholder *)
-Definition own_kvclerk (kck:loc) (γrpc:rpc_names): iProp Σ := True.
+Definition own_kvclerk (kck ks_srv:loc) (γrpc:rpc_names): iProp Σ := True.
 
-Definition is_kvserver := is_server (Server_own_core:=KVServer_own_core).
+Definition is_kvserver (srv:loc) γ := is_server (Server_own_core:=KVServer_own_core γ) srv γ.(ks_rpcGN).
 
-Lemma put_core_spec (srv:loc) (k:u64) (v:u64) :
+Lemma put_core_spec (srv:loc) (k:u64) (v:u64) γ :
 {{{ 
-     KVServer_own_core srv ∗ Put_Pre k v
+     KVServer_own_core γ srv ∗ k [[γ.(ks_kvMapGN)]]↦ _
 }}}
   KVServer__put_core #srv (#k, (#v, #()))%V
 {{{
-   RET #0; KVServer_own_core srv
-      ∗ (Put_Post k v)
+   RET #0; KVServer_own_core γ srv
+      ∗ k [[γ.(ks_kvMapGN)]]↦ v
 }}}.
 Proof.
   iIntros (Φ) "[Hksown Hpre] Hpost".
@@ -70,14 +75,14 @@ Proof.
   iFrame. iExists _, _; iFrame.
 Qed.
 
-Lemma get_core_spec (srv:loc) (k:u64) :
+Lemma get_core_spec (srv:loc) (k:u64) γ :
 {{{ 
-     KVServer_own_core srv ∗ Get_Pre k
+     KVServer_own_core γ srv ∗ k [[γ.(ks_kvMapGN)]]↦ _
 }}}
   KVServer__get_core #srv #k%V
 {{{
-   v, RET v; ∃va:u64, ⌜v = #va⌝ ∗ KVServer_own_core srv
-      ∗ (Get_Post k va)
+   v, RET v; ∃va:u64, ⌜v = #va⌝ ∗ KVServer_own_core γ srv
+      ∗ k [[γ.(ks_kvMapGN)]]↦ va
 }}}.
 Proof.
   iIntros (Φ) "[Hksown Hpre] Hpost".
@@ -106,25 +111,27 @@ Proof.
   iSplit; eauto. iExists _, _; iFrame.
 Qed.
 
-Lemma KVClerk__Get_spec (kck:loc) (key:u64) γ :
+Lemma KVClerk__Get_spec (kck ksrv:loc) (key:u64) γ :
 {{{
-     own_kvclerk kck γ ∗ (key [[γkv]]↦ _ )
+     is_kvserver ksrv γ ∗
+     own_kvclerk kck ksrv γ.(ks_rpcGN) ∗ (key [[γ.(ks_kvMapGN)]]↦ _ )
 }}}
   KVClerk__Get #kck #key
 {{{
      v, RET v; ∃va, 
-     own_kvclerk kck γ ∗ (key [[γkv]]↦ va )
+     own_kvclerk kck ksrv γ.(ks_rpcGN) ∗ (key [[γ.(ks_kvMapGN)]]↦ va )
 }}}.
 Admitted.
 
-Lemma KVClerk__Put_spec (kck:loc) (key va:u64) γ :
+Lemma KVClerk__Put_spec (kck ksrv:loc) (key va:u64) γ :
 {{{
-     own_kvclerk kck γ ∗ (key [[γkv]]↦ _ )
+     is_kvserver ksrv γ ∗
+     own_kvclerk kck ksrv γ.(ks_rpcGN) ∗ (key [[γ.(ks_kvMapGN)]]↦ _ )
 }}}
   KVClerk__Get #kck #key #va
 {{{
      RET #();
-     own_kvclerk kck γ ∗ (key [[γkv]]↦ va)
+     own_kvclerk kck ksrv γ.(ks_rpcGN) ∗ (key [[γ.(ks_kvMapGN)]]↦ va )
 }}}.
 Admitted.
 
