src/program_proof/lockservice/bank_proof.v
@@ -1,0 +1,60 @@
+From Coq.Structures Require Import OrdersTac.
+From stdpp Require Import gmap.
+From iris.algebra Require Import numbers.
+From iris.program_logic Require Export weakestpre.
+From Perennial.goose_lang Require Import prelude.
+From Perennial.goose_lang Require Import ffi.disk_prelude.
+From Perennial.goose_lang Require Import notation.
+From Perennial.program_proof Require Import proof_prelude.
+From RecordUpdate Require Import RecordUpdate.
+From Perennial.algebra Require Import auth_map fmcounter.
+From Perennial.goose_lang.lib Require Import lock.
+From Perennial.Helpers Require Import NamedProps.
+From Perennial.Helpers Require Import ModArith.
+From Perennial.program_proof.lockservice Require Import lockservice fmcounter_map rpc common_proof nondet rpc proof kv_proof.
+
+Record bank_names := BankGN {
+  bank_ls_names : lockservice_names;
+  bank_ks_names : kvservice_names;
+  bank_logBalGN : gname (* *)
+}.
+
+Class bankG Σ := BankG {
+  bank_ls :> lockserviceG Σ;
+  bank_ks :> kvserviceG Σ;
+  bank_logBalG :> mapG Σ u64 u64
+}.
+
+Section bank_proof.
+Context `{!heapG Σ, !bankG Σ}.
+
+Implicit Types (γ : bank_names).
+
+Context `{acc1:u64, acc2:u64}. (* Per-lock invariant *)
+
+Definition kv_gn γ := γ.(bank_ks_names).(ks_kvMapGN).
+Definition log_gn γ := γ.(bank_logBalGN).
+
+(* TODO: consider making is_*server part of own_*clerk *)
+Definition own_bank_clerk (bank_ck:loc) γ : iProp Σ :=
+  ∃ (lck kck ls_srv ks_srv:loc), 
+  "#Hls" ∷ is_lockserver ls_srv γ.(bank_ls_names) (Ps:=λ k, (∃v, k [[kv_gn γ]]↦v ∗ k [[log_gn γ]]↦v) )∗
+  "#Hks" ∷ is_kvserver ks_srv γ.(bank_ks_names) ∗
+  "Hlck_own" ∷ own_clerk #lck ls_srv γ.(bank_ls_names).(ls_rpcGN) ∗
+  "Hkck_own" ∷ own_kvclerk kck ks_srv γ.(bank_ks_names).(ks_rpcGN) ∗
+
+  "Hkck" ∷ bank_ck ↦[BankClerk.S :: "kvck"] #kck ∗
+  "Hlck" ∷ bank_ck ↦[BankClerk.S :: "lck"] #lck ∗
+  "Hacc1" ∷ bank_ck ↦[BankClerk.S :: "acc1"] #acc1 ∗
+  "Hacc1" ∷ bank_ck ↦[BankClerk.S :: "acc2"] #acc2 ∗
+
+  "#Hacc1_is_lock" ∷ lockservice_is_lock γ.(bank_ls_names) acc1 ∗
+  "#Hacc2_is_lock" ∷ lockservice_is_lock γ.(bank_ls_names) acc2
+.
+
+Definition bank_inv γ : iProp Σ :=
+  ∃ logBalMap:gmap u64 u64,
+  "HlogBalCtxl" ∷ map_ctx (log_gn γ) 1 logBalMap
+  .
+
+End bank_proof.
